Change types of stack slots to quantities
Replace the `ty` type field in stack slots with a `q` quantity field. The
idea is to make typing more coarse-grained, similarly to registers. This
solves some problems related to copying data between strictly typed slots
and more liberally typed registers.

This patch contains the target-independent parts of this change, as well as
the target-dependent parts for ARM.

common/PrintAST.ml
@@ -15,6 +15,7 @@
 open Printf
 open Camlcoq
 open AST
+open Memdata
 
 let name_of_type = function
   | Tint -> "int"
@@ -23,6 +24,10 @@ let name_of_type = function
   | Tsingle -> "single"
   | Tany32 -> "any32"
   | Tany64 -> "any64"
+
+let name_of_quantity = function
+  | Q32 -> "Q32"
+  | Q64 -> "Q64"
 
 let name_of_chunk = function
   | Mint8signed -> "int8s"
